stage commit

src/simple-proof/proof/Safety.v
@@ -64,15 +64,273 @@ Proof with auto.
       apply IHds...
 Qed.
 
-Lemma open_rec_eval_to_open_rec : forall k e x t t' L,
-  x \notin L ->
-  e[ open_rec_trm k x t |-> t'] ->
-  exists f, (x \notin (fv_trm f)) /\ t' = open_rec_trm k x f.
+Lemma open_lc_let_body : forall k t u x,
+    k >= 1 ->
+    lc_trm (trm_let t u) ->
+    open_rec_trm k x u = u.
 Proof.
-  intros. generalize dependent k.
-  generalize dependent e. generalize dependent x.
-  generalize dependent t'. generalize dependent L.
-  induction t; intros; try (solve [inversion H0]).
+  introv Hk H. inversion H.
+  specialize (H3 x).
+  pose proof H3 as H4.
+  apply lc_opening with (n:=k) (x:=x) in H3.
+  eapply (proj1 (lc_open_rec_open_trm_val_def_defs x _)).
+  - intro Contra. instantiate (1 := 0) in Contra. Coq.omega.Omega.omega.
+  - eassumption.
+Qed.
+Hint Resolve open_lc_let_body.      
+
+
+Definition close_rec_avar k u a : avar :=
+  match a with
+  | avar_b i => avar_b i
+  | avar_f x => If x = u then avar_b k else avar_f x
+  end.
+Hint Unfold close_rec_avar.
+
+Fixpoint close_rec_typ (k: nat) (u: var) (T: typ): typ :=
+  match T with
+  | typ_top        => typ_top
+  | typ_bot        => typ_bot
+  | typ_rcd D      => typ_rcd (close_rec_dec k u D)
+  | typ_and T1 T2  => typ_and (close_rec_typ k u T1) (close_rec_typ k u T2)
+  | typ_sel x L    => typ_sel (close_rec_avar k u x) L
+  | typ_bnd T      => typ_bnd (close_rec_typ (S k) u T)
+  | typ_all T1 T2  => typ_all (close_rec_typ k u T1) (close_rec_typ (S k) u T2)
+  end
+with close_rec_dec (k: nat) (u: var) (D: dec): dec :=
+  match D with
+  | dec_typ L T U => dec_typ L (close_rec_typ k u T) (close_rec_typ k u U)
+  | dec_trm m T   => dec_trm m (close_rec_typ k u T)
+  end.
+Hint Unfold close_rec_typ close_rec_dec.
+
+
+Fixpoint close_rec_trm (k: nat) (u: var) (t: trm): trm :=
+  match t with
+  | trm_var a      => trm_var (close_rec_avar k u a)
+  | trm_val v      => trm_val (close_rec_val k u v)
+  | trm_sel v m    => trm_sel (close_rec_avar k u v) m
+  | trm_app f a    => trm_app (close_rec_avar k u f) (close_rec_avar k u a)
+  | trm_let t1 t2  => trm_let (close_rec_trm k u t1) (close_rec_trm (S k) u t2)
+  end
+with close_rec_val (k: nat) (u: var) (v: val): val :=
+  match v with
+  | val_new T ds   => val_new (close_rec_typ (S k) u T) (close_rec_defs (S k) u ds)
+  | val_lambda T e => val_lambda (close_rec_typ k u T) (close_rec_trm (S k) u e)
+  end
+with close_rec_def (k: nat) (u: var) (d: def): def :=
+  match d with
+  | def_typ L T => def_typ L (close_rec_typ k u T)
+  | def_trm m e => def_trm m (close_rec_trm k u e)
+  end
+with close_rec_defs (k: nat) (u: var) (ds: defs): defs :=
+  match ds with
+  | defs_nil       => defs_nil
+  | defs_cons tl d => defs_cons (close_rec_defs k u tl) (close_rec_def k u d)
+  end.
+Hint Unfold close_rec_trm close_rec_val close_rec_def close_rec_defs.
+
+Definition close_avar u a := close_rec_avar  0 u a.
+Definition close_typ  u t := close_rec_typ   0 u t.
+Definition close_dec  u D := close_rec_dec   0 u D.
+Definition close_trm  u e := close_rec_trm   0 u e.
+Definition close_val  u v := close_rec_val   0 u v.
+Definition close_def  u d := close_rec_def   0 u d.
+Definition close_defs u l := close_rec_defs  0 u l.
+Hint Unfold close_avar close_typ close_dec close_trm close_val close_def close_defs.
+
+
+Lemma close_rec_typ_dec_no_capture : forall x,
+    (forall T k, x \notin fv_typ (close_rec_typ k x T)) /\
+    (forall D k, x \notin fv_dec (close_rec_dec k x D)).
+Proof.
+  intros x. apply typ_mutind; intros; simpl; auto;
+  destruct a; simpl;
+  try case_if; unfold fv_avar; auto.
+Qed.
+
+
+Lemma close_rec_trm_val_def_defs_no_capture: forall x,
+    (forall t k, x \notin fv_trm (close_rec_trm k x t)) /\
+    (forall v k, x \notin fv_val (close_rec_val k x v)) /\
+    (forall d k, x \notin fv_def (close_rec_def k x d)) /\
+    (forall ds k, x \notin fv_defs (close_rec_defs k x ds)).
+Proof.
+  intro x.
+  apply trm_mutind; intros; simpl; auto;
+    try apply notin_union;
+    repeat split;
+    try applys close_rec_typ_dec_no_capture;
+    repeat
+      match goal with
+      | [ |- _ \notin fv_avar (close_rec_avar _ _ ?a) ] => destruct a; simpl
+      | [ |- _ \notin fv_avar (close_rec_avar _ _ ?a) \u _ ] => destruct a; simpl
+      | [ |- _ \notin _ \u fv_avar (close_rec_avar _ _ ?a) ] => destruct a; simpl
+      end;
+    repeat case_if; unfold fv_avar; auto.
+Qed.  
+  
+
+(* Ltac optrm_struct H := *)
+(*   (try match type of H with *)
+(*        | open_trm _ _ => unfold open_trm in H *)
+(*        end); *)
+(*   (try match type of H with *)
+(*        | _ = open_rec_trm _ _ _ => symmetry in H *)
+(*        end); *)
+(*   match type of H with *)
+(*   | open_rec_trm _ _ ?t = _ => destruct t; simpl in H; inversion H *)
+(*   end. *)
+
+(* Lemma open_rec_eval_to_open_rec : forall k e x t t' v, *)
+(*     x \notin dom e \u fv_trm t \u fv_val v -> *)
+(*     lc_sto e -> lc_val v -> *)
+(*     e & x ~ v[ open_rec_trm k x t |-> t'] -> *)
+(*     exists f, (* (x \notin (fv_trm f)) /\ *) t' = open_rec_trm k x f. *)
+(* Proof. *)
+  (* intros. gen k e x t' v. *)
+  (* induction t; intros; inversion H2; subst. *)
+  (*   (* try solve [ *) *)
+  (*   (*       match goal with *) *)
+  (*   (*       | [ H : _ [ _ |-> _ ] |- _ ] => inversion H *) *)
+  (*   (*       end]. *) *)
+  (* - pose proof H9 as Hop. *)
+  (*   apply open_rec_defs_has_open_rec_trm in H9. destruct_all. subst. *)
+  (*   apply binds_push_inv in H7; destruct_all; subst; *)
+  (*     repeat *)
+  (*       match goal with *)
+  (*       | [ H : binds _ _ e |- _ ] => apply lc_sto_binds_inv in H; auto *)
+  (*       | [ H : lc_val (val_new _ _) |- _ ] => inversion H; clear H; subst *)
+  (*       | [ H : forall _, lc_defs _, *)
+  (*             Hdefs : defs_has (open_defs ?x _) _ |- _ ] => *)
+  (*         specialize (H x); apply (lc_defs_has H) in Hdefs; inversion Hdefs; subst *)
+  (*       end; *)
+  (*     eexists; rewrite (proj1 (lc_opening_trm_val_def_defs _)) with (n:=k); auto. *)
+  (* - apply binds_push_inv in H8; destruct_all; subst; *)
+  (*     repeat *)
+  (*       match goal with *)
+  (*       | [ H : binds _ _ e |- _ ] => apply lc_sto_binds_inv in H; auto *)
+  (*       | [ H : lc_val (val_lambda _ _) |- _ ] => inversion H; clear H *)
+  (*       | [ H : forall _, lc_trm _ |- _ ] => specialize (H y) *)
+  (*       end; *)
+  (*     eexists; rewrite (proj1 (lc_opening_trm_val_def_defs x)); auto. *)
+  (* - optrm_struct H3. unfold open_rec_avar in H5. *)
+
+(* Lemma open_rec_eval_to_open_rec : forall e x t t' v, *)
+(*     x \notin dom e \u fv_trm t \u fv_val v -> *)
+(*     lc_sto e -> lc_val v -> *)
+(*     e & x ~ v[ open_trm x t |-> t'] -> *)
+(*     exists f, (x \notin (fv_trm f)) /\ t' = open_trm x f. *)
+(* Proof. *)
+(*   intros. gen e x t' v. *)
+(*   induction t; intros; inversion H2; subst. *)
+(*     (* try solve [ *) *)
+(*     (*       match goal with *) *)
+(*     (*       | [ H : _ [ _ |-> _ ] |- _ ] => inversion H *) *)
+(*     (*       end]. *) *)
+(*   - pose proof H9 as Hop. *)
+(*     apply open_rec_defs_has_open_rec_trm in H9. destruct_all. subst. *)
+(*     apply binds_push_inv in H7; destruct_all; subst; *)
+(*       repeat *)
+(*         match goal with *)
+(*         | [ H : binds _ _ e |- _ ] => apply lc_sto_binds_inv in H; auto *)
+(*         | [ H : lc_val (val_new _ _) |- _ ] => inversion H; clear H; subst *)
+(*         | [ H : forall _, lc_defs _, *)
+(*               Hdefs : defs_has (open_defs ?x _) _ |- _ ] => *)
+(*           specialize (H x); apply (lc_defs_has H) in Hdefs; inversion Hdefs; subst *)
+(*         end. *)
+(*     + exists x1. *)
+    
+  (*     match goal with *)
+  (*     | [ |- exists _, _ /\ ?l = (open_trm ?x _) ] => exists l; split; *)
+  (*                                               [ |symmetry; *)
+  (*                                               apply (proj1 (lc_opening_trm_val_def_defs x)); auto] *)
+  (*     end. *)
+  (* - apply binds_push_inv in H8; destruct_all; subst; *)
+  (*     repeat *)
+  (*       match goal with *)
+  (*       | [ H : binds _ _ e |- _ ] => apply lc_sto_binds_inv in H; auto *)
+  (*       | [ H : lc_val (val_lambda _ _) |- _ ] => inversion H; clear H *)
+  (*       | [ H : forall _, lc_trm _ |- _ ] => specialize (H y) *)
+  (*       end; *)
+  (*     match goal with *)
+  (*     | [ |- exists _, ?l = (open_trm ?x _) ] => exists l; symmetry; *)
+  (*                                           apply (proj1 (lc_opening_trm_val_def_defs x)); auto *)
+  (*     end. *)
+  (* - inversion H7. specialize (H8 y). *)
+  (*   match goal with *)
+  (*   | [ |- exists _, ?l = (open_trm ?x _) ] => exists l; symmetry; *)
+  (*                                         apply (proj1 (lc_opening_trm_val_def_defs x)); auto *)
+  (*   end. *)
+  (* - *)
+    
+
+    
+  (* introv Hx Hlce Hlcv He. dependent induction He. *)
+  (* - exists (open_trm y t0). *)
+  (*   split. *)
+  (*   + admit. *)
+  (*   + *)
+  (*   apply binds_push_inv in H0; destruct_all; subst; *)
+  (*     repeat *)
+  (*       match goal with *)
+  (*       | [ H : binds _ _ e |- _ ] => apply lc_sto_binds_inv in H; auto *)
+  (*       | [ H : lc_val (val_lambda _ _) |- _ ] => inversion H; clear H *)
+  (*       | [ H : forall _, lc_trm _ |- _ ] => specialize (H y) *)
+  (*       end; *)
+  (*     rewrite (proj1 (lc_opening_trm_val_def_defs x1)); auto. *)
+  (* - admit. *)
+  (*   (* pose proof H1. apply open_rec_defs_has_open_rec_trm in H1. *) *)
+  (*   (* apply binds_push_inv in H0; destruct_all; subst; *) *)
+  (*   (*   repeat *) *)
+  (*   (*     match goal with *) *)
+  (*   (*     | [ H : binds _ _ e |- _ ] => apply lc_sto_binds_inv in H; auto *) *)
+  (*   (*     | [ H : lc_val (val_new _ _) |- _ ] => inversion H; clear H; subst *) *)
+  (*   (*     | [ H : forall _, lc_defs _, Hdefs : defs_has (open_defs ?x _) _ |- _ ] => *) *)
+  (*   (*       specialize (H x); apply (lc_defs_has H) in Hdefs; inversion Hdefs; subst *) *)
+  (*   (*     | [ |- exists _, open_rec_trm _ ?x ?t = open_rec_trm ?k ?y _ ] => *) *)
+  (*   (*       exists (open_trm x t); rewrite (proj1 (lc_opening_trm_val_def_defs y)) with (n:= k); auto *) *)
+  (*   (*     end. *) *)
+  (* - rename x into Hop. destruct t; simpl in Hop; inversion Hop. *)
+
+(*     admit. *)
+(*   - admit. *)
+(*   - admit. *)
+(*   - admit. *)
+(* Qed. *)
+  
+(*   intros. gen k e x t' v. induction t; intros. *)
+(*   - inversion H2. *)
+(*   - inversion H2. *)
+(*   - unfold open_rec_trm in H2. unfold open_rec_avar in H2. *)
+(*     destruct a; [case_if |]; inversion H2; subst. *)
+(*     + apply binds_push_eq_inv in H7. subst. *)
+(*       exists t'. destruct (open_rec_defs_has_open_rec_trm _ _ _ H9). *)
+(*       subst. *)
+
+
+(*       split. *)
+(*       * unfold fv_val in H. fold fv_defs in H. *)
+(*         assert (ds = open_defs x ds). { *)
+          
+(*         } *)
+    
+
+(*   (*   inversion H0. subst. *) *)
+    
+(*   (* intros. dependent induction H0; intros. *) *)
+(*   (* - exists t. split; auto. *) *)
+    
+  
+(* Lemma open_rec_eval_to_open_rec : forall e x t t' v, *)
+(*   x \notin dom e \u fv_trm t \u fv_val v -> *)
+(*   e & x ~ v[ open_trm x t |-> t'] -> *)
+(*   exists f, (x \notin (fv_trm f)) /\ t' = open_trm x f. *)
+(* Proof. *)
+(*   introv Hx He. dependent induction He. *)
+(*   -  *)
+  
+(*   (* induction t; intros; try (solve [inversion H0]). *) *)
 Admitted.
 
 Lemma subenv_empty_supremum : forall G, subenv G empty.
@@ -160,23 +418,7 @@ Proof.
 Qed.
 Hint Resolve indc_subenv_push.
 
-Lemma open_lc_let_body : forall k t u x,
-    k >= 1 ->
-    lc_trm (trm_let t u) ->
-    open_rec_trm k x u = u.
-Proof.
-  introv Hk H. inversion H.
-  specialize (H3 x).
-  pose proof H3 as H4.
-  apply lc_opening with (n:=k) (x:=x) in H3.
-  eapply (proj1 (lc_open_rec_open_trm_val_def_defs x _)).
-  - intro Contra. instantiate (1 := 0) in Contra. Coq.omega.Omega.omega.
-  - eassumption.
-Qed.
-Hint Rewrite open_lc_let_body.
-Hint Resolve open_lc_let_body.      
-  
-  
+
 Lemma eval_renaming: forall x y e t t1 t2,
     x \notin (dom e) \u (fv_val t) \u (fv_trm t1) \u (fv_trm t2) ->
     (e & x ~ t)[ open_trm x t1 |-> open_trm x t2 ] ->
@@ -186,6 +428,7 @@ Proof. Admitted.
  
 
 Lemma progress_ec: forall G' G e t T,
+    lc_sto e ->
     lc_trm t ->
     indc_subenv G' G ->
     inert G' ->
@@ -194,7 +437,7 @@ Lemma progress_ec: forall G' G e t T,
     ok G ->
     (normal_form t \/ exists t', e[t |-> t']).
 Proof with auto.
-  introv Hlc Hsenv Hig Hwf Ht Hokg. gen G' e.
+  introv Hlce Hlc Hsenv Hig Hwf Ht Hokg. gen G' e.
   induction Ht; eauto; intros.
   - Case "ty_all_elim".
     apply narrow_typing with (G':=G') in Ht1; auto.
@@ -210,33 +453,41 @@ Proof with auto.
       apply narrow_typing with (G':=G') in Ht; auto.
       destruct (var_typing_implies_avar_f Ht); subst.
       right. exists (open_trm x u). constructor...      
-    + apply val_typing in Ht.
+    + SCase "t = trm_val v".
+      apply val_typing in Ht.
       destruct Ht as [T' [H1 H2]].
       pose proof (precise_inert_typ H1) as Hpit.
       pick_fresh x.
       destruct H0 with (x:=x) (G' := G' & x ~ T') (e := e & x ~ v); auto.
       * inversion Hlc. trivial.
       * intros. eapply indc_subenv_trans; econstructor; eauto.
+      * constructor; auto. inversion Hlc. inversion H5. trivial.
       * intros. apply precise_to_general in H1.
         constructor; auto. eapply narrow_typing in H1; eauto.
       * left.
         destruct u; auto; apply open_preserve_normal_form in H3; auto.
       * right. destruct H3.
+
+        (* exists. eapply red_let_val; auto. *)
+        (* intros. *)
+        
+        
         pose proof H3.
-        apply (open_rec_eval_to_open_rec _ _ Fr) in H3.
-        destruct H3. destruct H3. subst.
+        apply open_rec_eval_to_open_rec in H3; auto.
+        destruct_all. subst.
         eexists. eapply red_let_val; auto.
         intros.
         eapply eval_renaming with (x:=x); eauto.
+        inversion Hlc. inversion H7. trivial.
     + SCase "t = trm_sel a t".
       right.
       inversion Hlc.
-      destruct (IHHt H3 Hokg G' Hsenv Hig e Hwf) as [Hnf | [t' Hr]]. inversion Hnf.
+      destruct (IHHt H3 Hokg G' Hsenv Hig e Hlce Hwf) as [Hnf | [t' Hr]]. inversion Hnf.
       eexists. constructor*.
     + SCase "t = trm_app a a0".
       right.
       inversion Hlc.
-      destruct (IHHt H3 Hokg G' Hsenv Hig e Hwf) as [Hnf | [t' Hr]]. inversion Hnf.
+      destruct (IHHt H3 Hokg G' Hsenv Hig e Hlce Hwf) as [Hnf | [t' Hr]]. inversion Hnf.
       eexists. constructor*.
     + SCase "t = trm_let t1 t2".
       right. eexists. constructor. inversion Hlc. trivial.
@@ -299,14 +550,11 @@ Proof.
          }
          rewrite H2. trivial.
     * SCase "red_let_let".
-      (* apply narrow_typing with (G':=G') in Ht; auto. *)
       clear H0 IHHt.
       assert (forall x, x \notin (L \u dom G) -> G & x ~ T ⊢ open_trm x u : U). {
         intros. assert (x \notin L); auto.
       }
       clear H.
-      
-      (* apply narrow_typing with (G' := G') in Ht; auto. *)
       dependent induction Ht.
       -- apply narrow_typing with (G' := G') in Ht; eauto.
          remember ((((((((((((L \u L0) \u dom G) \u fv_ctx_types G) \u dom G')
@@ -367,9 +615,6 @@ Proof.
       assert (x \notin L0); auto.
       inversion Hlc.
       specialize (H0 _ H3 (H14 _) H5 (G' & x ~ T') H7 H8 (e & x ~ v) H9 _ (H6 _ H10)).
-      (* remember ((((((((((((L \u L0) \u dom G) \u fv_ctx_types G) \u dom G') *)
-      (*                    \u fv_ctx_types G') \u dom e) \u fv_trm u) \u fv_trm t'0) *)
-      (*                \u fv_val v) \u fv_typ T) \u fv_typ U) \u fv_typ T') as bigL. *)
       apply_fresh ty_let as y; eauto.
 
       apply weaken_ty_trm with (G2:=(y ~ T')) in H0; auto.
